bring the patterns in accordance with the schemes and fix prove methods

Previous.thy
@@ -2,97 +2,122 @@ theory Previous
   imports Always
 begin
 
-definition weak_previous where " weak_previous s A \<equiv>
-\<forall> s1. consecutive s1 s \<longrightarrow> A s1"
+definition weak_previous where " weak_previous (s::state) s1 A \<equiv>
+\<forall> r1. consecutive r1 s1 \<longrightarrow> A s r1"
 
-definition previous where "previous s A \<equiv>
-\<exists> s1. consecutive s1 s \<and> A s1"
+definition previous where "previous (s::state) s1 A \<equiv>
+\<exists> r1. consecutive r1 s1 \<and> A s r1"
+
+definition previous_inv where "previous_inv (s::state) (A::state\<Rightarrow>state\<Rightarrow>bool) \<equiv> A s s"
 
 definition always2 where  "always2 s A1 A2 A3 \<equiv> 
-always s (\<lambda> s2.( previous s2 A1) \<and> A2 s2 \<longrightarrow> A3 s2)"
+always s s (\<lambda> r2 r1. weak_previous r2 r1 (\<lambda> r4 r3. \<not> A1 r3) \<or> \<not> A2 r1 \<or> A3 r2 r1)"
 
 definition always2_inv where  "always2_inv s b A1 A2 A3 \<equiv> 
-always s (\<lambda> s2.( previous s2 A1) \<and> A2 s2 \<longrightarrow> A3 s2) \<and> (b \<longrightarrow> \<not>A1 s)"
+always_inv s (\<lambda> r2 r1. weak_previous r2 r1 (\<lambda> r4 r3. \<not> A1 r3) \<or> \<not> A2 r1 \<or> A3 r2 r1)
+ \<and> (b s \<longrightarrow> previous_inv s (\<lambda> r2 r1. \<not> A1 r1))"
 
-lemma weak_previous_one_point: "consecutive s0 s \<Longrightarrow>  A s0 \<Longrightarrow> weak_previous s A"
-  apply(unfold  weak_previous_def)
+lemma weak_previous_one_point[patternintro]: "consecutive s s'
+ \<Longrightarrow> previous_inv s A \<and> always_imp s (A s) (A s')
+ \<Longrightarrow> weak_previous s' s' A"
+  unfolding previous_inv_def weak_previous_def always_imp_def
   apply simp
-  by (metis toEnvNum_eq_imp_eq2)
+  by (metis substate_refl toEnvNum_eq_imp_eq2)
 
-lemma previous_one_point: "consecutive s0 s \<Longrightarrow>  A s0  \<Longrightarrow> previous s A"
-  apply(unfold  previous_def)
+lemma previous_one_point[patternintro]: "consecutive s s' \<Longrightarrow> previous_inv s A \<and> always_imp s (A s) (A s')
+  \<Longrightarrow> previous s' s' A"
+  unfolding previous_inv_def previous_def always_imp_def
   by auto
 
-lemma previous_ex_not: "\<not> previous s A \<longleftrightarrow> weak_previous s (\<lambda> s0. \<not> A s0)"
-  using weak_previous_def previous_def by presburger
+lemma previous_rule[pastinv]: "consecutive s s' \<Longrightarrow> A s' s' \<Longrightarrow> previous_inv s' A"
+  unfolding previous_inv_def
+  by auto
 
-lemma always2_rule: "
-always2_inv s0 b A1 A2 A3 \<Longrightarrow>consecutive s0 s \<Longrightarrow> (((b \<or> ~ A2 s) \<or> A3' s) \<and> (\<forall> s1. toEnvP s1 \<and> substate s1 s0 \<and> A3 s1 \<longrightarrow> A3' s1)) \<and> (b' \<longrightarrow> \<not>A1 s) \<Longrightarrow>
- always2_inv s b' A1 A2 A3'"
-  apply(unfold always2_inv_def)
-  apply(simp only: imp_conv_disj de_Morgan_conj previous_ex_not )
-  apply(erule conjE)
+lemma weak_previous_LS4[invsaving]: "consecutive s s' \<Longrightarrow> always_imp s (A s) (A s') 
+\<Longrightarrow> always_imp s (\<lambda> s1. weak_previous s s1 A) (\<lambda> s1. weak_previous s' s1 A)"
+  unfolding weak_previous_def always_imp_def
+  apply simp
+  by (meson substate_trans)
+
+lemma weak_previous_LS5[inv_req]: "toEnvP s \<Longrightarrow> always_imp s (A' s) (A s) 
+\<Longrightarrow> always_imp s (\<lambda> s1. weak_previous s s1 A') (\<lambda> s1. weak_previous s s1 A)"
+  unfolding weak_previous_def always_imp_def
+  apply simp
+  using substate_trans by blast
+
+lemma always2_rule_gen: 
+"always2_inv s b A1 A2 A3 \<Longrightarrow> consecutive s s'
+ \<Longrightarrow> ((True \<and> True \<and>  always_imp s (A3 s) (A3 s')) \<and> (b s \<and> True \<or> \<not> A2 s' \<or> A3 s' s')) \<and> (b s' \<longrightarrow> \<not> A1 s')
+ \<Longrightarrow> always2_inv s' b A1 A2 A3"
+  unfolding always2_inv_def
+  apply(proveOuter add_rules: invsaving)
+  done
+ (* apply(erule conjE)
   apply(erule conjE)
   subgoal premises prems1
     apply(rule conjI)
      apply(insert prems1(1,2,4))[1]
-     apply(erule always_rule)
-      apply simp
+     apply(erule elims)
+      apply assumption
      apply(erule conjE)
     subgoal premises prems2
-      apply(rule conjI)
+       apply(rule conjI)
        apply(insert prems2(1,2))[1]
-       apply(erule disjE)
-        apply(rule disjI1)
-        apply(erule disjE)
-         apply(rule disjI1)
-         apply(rule weak_previous_one_point[of s0])
-      apply simp
-      using prems1(3) apply simp
-        apply(rule disjI2)
-        apply assumption 
-       apply(rule disjI2)
-       apply assumption
-      apply(insert prems2(1,3))[1]
-      apply auto
-      done
-    apply(insert prems1(1,3,5))
-    apply simp
-    done
-  done
-
-lemma always2_einv2req: "always2_inv s b A1 A2 A3 \<Longrightarrow>  (\<forall> s1. toEnvP s1 \<and> substate s1 s \<and> A3 s1 \<longrightarrow> A3' s1) \<Longrightarrow> always2 s A1 A2 A3'"
-  apply(unfold always2_def always2_inv_def)
-  by (metis (mono_tags, lifting) always_einv2req)
-
-definition always2_2 where  "always2_2 s A1 A2 A3 \<equiv> 
-always2 s A1 A2 (\<lambda> s2. weak_previous s2 (\<lambda> s1. A3 s1 s2))"
-
-definition always2_2_inv where  "always2_2_inv s b A1 A2 A3 \<equiv> 
-always2_inv s b A1 A2 (\<lambda> s2. weak_previous s2 (\<lambda> s1. A3 s1 s2))"
-
-lemma always2_2_rule: "
-always2_2_inv s0 b A1 A2 A3 \<Longrightarrow>consecutive s0 s \<Longrightarrow> (((b \<or> ~ A2 s) \<or> A3 s0 s) ) \<and> (b' \<longrightarrow> \<not>A1 s) \<Longrightarrow>
- always2_2_inv s b' A1 A2 A3"
-  apply(unfold always2_2_inv_def)
-  apply(erule always2_rule)
-   apply simp
-  apply(erule conjE)
-  subgoal premises prems1
-    apply(rule conjI)
-     apply(insert prems1(1,2))[1]
-     apply(rule conjI)
+       apply(rule patternintro)
+        apply simp
+       apply(erule conjE)
+      subgoal premises prems3
+        apply(rule conjI)
+         apply(insert prems3(1,2))[1]
+         apply(rule invsaving)
+          apply assumption
+        apply prove
+        apply(insert prems3(1,3))
+        apply(rule patternintro)
+         apply simp
+        apply(erule conjE)
+        subgoal premises prems4
+          apply(rule conjI)
+           apply(insert prems4(1,2))[1]
+           apply(rule always_imp_refl)
+          apply(insert prems4(1,3))
+          apply assumption
+          done
+        done
+      apply(insert prems2(1,3))
       apply(erule disjE)
        apply(rule disjI1)
-       apply simp
+       apply(rule patternintro)
+        apply assumption
+       apply(erule conjE)
+      subgoal premises prems3
+        apply(rule conjI)
+         apply(insert prems3(1,2))[1]
+         apply(rule mp[OF prems1(3) prems3(2)])
+        apply(insert prems3(1,3))
+        apply(rule always_imp_refl)
+        done
       apply(rule disjI2)
-      apply(rule weak_previous_one_point[of s0])
-       apply simp
-      apply simp
-     apply simp
-    apply(insert prems1(1,3))
-    apply simp
+      apply assumption
+      done
+    apply(insert prems1(1,5))
+    apply(rule impI)
+    apply(erule impE)
+     apply assumption
+    subgoal premises prems2
+      apply(insert prems2(1,3))
+      apply(rule pastinv)
+       apply assumption
+      apply assumption
+      done
     done
   done
-
+*)
+        
 end
+
+
+
+
+
+
