RequirementLemmas.thy
@@ -26,7 +26,7 @@ lemma always_imp_refl: " always_imp s A A"
   apply(unfold always_imp_def)
   by auto
 
-method prove =
+method prove declares add_rules einvs =
 (*formula without requirement and extra invariant patterns*)
 assumption |
 (*conjunction*)
@@ -39,15 +39,19 @@ match premises in e[thin]: _ (cut) \<Rightarrow>
 match conclusion in "?P \<or> ?Q" \<Rightarrow> \<open>erule disjE,rule disjI1,prove,rule disjI2,prove\<close> |
 (*implication*)
 match conclusion in "?b \<longrightarrow> ?P" \<Rightarrow>
-\<open>rule impI,rule impE,assumption,rotate_tac,match premises in p[thin]: _ (cut) \<Rightarrow> \<open>rotate_tac,prove\<close>\<close> |
+\<open>rule impI,rule impE,assumption,
+match premises in e[thin]: _ (cut) \<Rightarrow>
+\<open>match premises in b[thin]: _ (cut) \<Rightarrow>
+\<open>match premises in p[thin]: _ (cut) \<Rightarrow>
+ \<open>(insert e p)[1];prove\<close>\<close>\<close>\<close> |
 (*\<forall> s1. e(s1) \<and> s1 \<le> s \<and> A(s1) \<longrightarrow> A'(s1)*)
-match conclusion in "always_imp ?s ?A ?A'" \<Rightarrow> \<open>fact always_imp_refl\<close> |
+match conclusion in "always_imp ?s ?A ?A" \<Rightarrow> \<open>rule always_imp_refl\<close> |
 (*pattern*)
 rule patternintro add_rules,(assumption | simp),prove |
 (*past extra invariant pattern*)
 rotate_tac;match premises in p[thin]: b (cut) for b \<Rightarrow> \<open>match einvs in i: "b \<longrightarrow> ?P" \<Rightarrow> \<open>fact mp[OF i p]\<close>\<close>
 
-method proveOuter declares add_rules =
+method proveOuter declares add_rules einvs =
 (*conjunction*)
 match conclusion in "?P \<and> ?Q" \<Rightarrow>
 \<open>erule conjE;erule conjE;
@@ -59,22 +63,28 @@ match premises in e[thin]: _ (cut) \<Rightarrow>
 \<open>rule conjI,(insert e i1 p1)[1],proveOuter,(insert e i2 p2)[1],proveOuter\<close>\<close>\<close>\<close>\<close>\<close> |
 (*disjunction*)
 match conclusion in "?P \<or> ?Q" \<Rightarrow>
-\<open>erule conjE;rotate_tac 2;
+\<open>erule conjE;
 match premises in p1[thin]: _ (cut) \<Rightarrow>
 \<open>match premises in p2[thin]: _ (cut) \<Rightarrow>
-\<open>erule disjE,(insert p1)[1],rule disjI1,proveOuter,(insert p2)[1],rule disjI2,proveOuter\<close>\<close>\<close> |
+\<open>match premises in p3[thin]: _ (cut) \<Rightarrow>
+\<open>match premises in p4[thin]: _ (cut) \<Rightarrow>
+\<open>(insert p1 p2)[1],erule disjE,(insert p3)[1],rule disjI1,proveOuter,(insert p4)[1],rule disjI2,proveOuter\<close>\<close>\<close>\<close>\<close> |
 (*implication: additional conjunct*)
 match conclusion in "?b \<longrightarrow> ?P" \<Rightarrow>
-\<open>rotate_tac;
-match premises in i[thin]: _ (cut) \<Rightarrow>
-\<open>rule impI,erule impE,assumption,rotate_tac,
-match premises in b[thin]: _ (cut) \<Rightarrow>
-\<open>rotate_tac,rule pastinv,assumption,prove\<close>\<close>\<close> |
+\<open>match premises in e[thin]: _ (cut) \<Rightarrow>
+\<open>match premises in i[thin]: _ (cut) \<Rightarrow>
+\<open>match premises in p[thin]: _ (cut) \<Rightarrow>
+\<open>(insert e p)[1],rule impI,erule impE,assumption,
+match premises in e[thin]: _ (cut) \<Rightarrow>
+\<open>match premises in b[thin]: _ (cut) \<Rightarrow>
+\<open>match premises in p[thin]: _ (cut) \<Rightarrow>
+\<open>(insert e p)[1],rule pastinv,assumption,prove\<close>\<close>\<close>\<close>\<close>\<close>\<close> |
 (*pattern*)
-rotate_tac -1;
-match premises in p[thin]: _ (cut) \<Rightarrow>
-\<open>(simp only: conj_assoc)?;
+match premises in p1[thin]: _ (cut) \<Rightarrow>
+\<open>match premises in p2[thin]: _ (cut) \<Rightarrow>
+\<open>match premises in p3[thin]: _ (cut) \<Rightarrow>
+\<open>(insert p1 p2)[1];(simp only: conj_assoc)?;
 (erule conjE;rotate_tac -1;match premises in ac[thin]: _ (cut) \<Rightarrow> \<open>succeed\<close>)?;
-erule elims,assumption,(insert p)[1],prove\<close>
+erule elims,assumption,(insert p3)[1],prove\<close>\<close>\<close>
 
 end
